@prefix : <http://morelab.deusto.es/ontologies/riskC4A#> .
@prefix owl: <http://www.w3.org/2002/07/owl#> .
@prefix rdf: <http://www.w3.org/1999/02/22-rdf-syntax-ns#> .
@prefix xml: <http://www.w3.org/XML/1998/namespace> .
@prefix xsd: <http://www.w3.org/2001/XMLSchema#> .
@prefix rdfs: <http://www.w3.org/2000/01/rdf-schema#> .
@base <http://morelab.deusto.es/ontologies/riskC4A> .

<http://morelab.deusto.es/ontologies/riskC4A> rdf:type owl:Ontology .

#################################################################
#    Object Properties
#################################################################

###  http://morelab.deusto.es/ontologies/riskC4A#hasCategories
:hasCategories rdf:type owl:ObjectProperty ;
               rdfs:domain :Instrument ;
               rdfs:range :Category .


###  http://morelab.deusto.es/ontologies/riskC4A#hasItems
:hasItems rdf:type owl:ObjectProperty ;
          rdfs:domain :Category ;
          rdfs:range :Item .


###  http://morelab.deusto.es/ontologies/riskC4A#hasModel
:hasModel rdf:type owl:ObjectProperty ;
          rdfs:domain :Instrument ;
          rdfs:range :Model .


###  http://morelab.deusto.es/ontologies/riskC4A#hasScore
:hasScore rdf:type owl:ObjectProperty ;
          rdfs:domain :Instrument ,
                      :Item ;
          rdfs:range :Score .


###  http://morelab.deusto.es/ontologies/riskC4A#hasValue
:hasValue rdf:type owl:ObjectProperty ;
          rdfs:domain :Item ;
          rdfs:range :Value .


###  http://morelab.deusto.es/ontologies/riskC4A#hasValues
:hasValues rdf:type owl:ObjectProperty ;
           rdfs:domain :Model ;
           rdfs:range :Value .


#################################################################
#    Classes
#################################################################

###  http://morelab.deusto.es/ontologies/riskC4A#Category
:Category rdf:type owl:Class ;
          rdfs:comment "Group of Items (see below) that contribute to the appraisal of a certain facet of the measured health entity."^^xsd:string .


###  http://morelab.deusto.es/ontologies/riskC4A#Instrument
:Instrument rdf:type owl:Class ;
            rdfs:comment "Overall measuring method, aimed at providing a final, comprehensive score on a certain health entity."^^xsd:string .


###  http://morelab.deusto.es/ontologies/riskC4A#Interval
:Interval rdf:type owl:Class ;
          rdfs:subClassOf :Score ;
          rdfs:comment "Difference among numbers is meaningful like the concept of unit of measure (e.g. temperature in ºC)."^^xsd:string .


###  http://morelab.deusto.es/ontologies/riskC4A#Item
:Item rdf:type owl:Class ;
      rdfs:comment "Each actual, basic element that will be measured to produce scores."^^xsd:string .


###  http://morelab.deusto.es/ontologies/riskC4A#Model
:Model rdf:type owl:Class ;
       rdfs:comment "Mathematical entity (algorithms and/or calculations) that allows to compute the Instrument outcome score on the basis of the scores measured for single Items."^^xsd:string .


###  http://morelab.deusto.es/ontologies/riskC4A#Nominal
:Nominal rdf:type owl:Class ;
         rdfs:subClassOf :Score ;
         rdfs:comment "Numbers are used just as labels for categories (e.g. 0 for false and 1 for true, for a classifier outcome)."^^xsd:string .


###  http://morelab.deusto.es/ontologies/riskC4A#Ordinal
:Ordinal rdf:type owl:Class ;
         rdfs:subClassOf :Score ;
         rdfs:comment "Order is meaningful and represents growing quantities (e.g. 1 = mild, 2 = moderate, 3 = strong)."^^xsd:string .


###  http://morelab.deusto.es/ontologies/riskC4A#Ratio
:Ratio rdf:type owl:Class ;
       rdfs:subClassOf :Score ;
       rdfs:comment "There is a meaningful zero point, so ratios among scores are also meaningful (e.g. number of seconds to complete an action)."^^xsd:string .


###  http://morelab.deusto.es/ontologies/riskC4A#Score
:Score rdf:type owl:Class ;
       rdfs:comment "The outcome of measuring an Item (or the outcome of the overall Instrument)."^^xsd:string .


###  http://morelab.deusto.es/ontologies/riskC4A#Value
:Value rdf:type owl:Class ;
       rdfs:comment "Set of values associated to an Item. The Item’s measurement produces a specific score, drawn from this set."^^xsd:string .


###  Generated by the OWL API (version 5.1.0) https://github.com/owlcs/owlapi/
